thys/Buchi_Complementation/Complementation_Implement.thy
@@ -69,13 +69,11 @@ begin
     "('label, 'state) nba \<Rightarrow> 'label \<Rightarrow> 'state items \<Rightarrow> 'state items set" where
     "complement_succ_1 A a = ranks_1 A a \<circ> refresh_1"
   definition complement_1 :: "('label, 'state) nba \<Rightarrow> ('label, 'state items) nba" where
-    "complement_1 A \<equiv>
-    \<lparr>
-      alphabet = alphabet A,
-      initial = {const (Some (2 * card (nodes A), False)) |` initial A},
-      succ = complement_succ_1 A,
-      accepting = \<lambda> f. cs_st f = {}
-    \<rparr>"
+    "complement_1 A \<equiv> nba
+      (alphabet A)
+      ({const (Some (2 * card (nodes A), False)) |` initial A})
+      (complement_succ_1 A)
+      (\<lambda> f. cs_st f = {})"
 
   lemma refresh_1_dom[simp]: "dom (refresh_1 f) = dom f" unfolding refresh_1_def by simp
   lemma refresh_1_apply[simp]: "fst (the (refresh_1 f p)) = fst (the (f p))"
@@ -198,11 +196,11 @@ begin
       show "cs_abs g \<in> complement_succ A a (cs_abs f)" using complement_succ_1_abs 1 by this
     qed
   qed
-  lemma complement_1_refine: "(complement_1, complement) \<in> \<langle>Id, Id, Id\<rangle> nba_rel \<rightarrow> \<langle>Id, cs_rel, Id\<rangle> nba_rel"
+  lemma complement_1_refine: "(complement_1, complement) \<in> \<langle>Id, Id\<rangle> nba_rel \<rightarrow> \<langle>Id, cs_rel\<rangle> nba_rel"
   unfolding complement_1_def complement_def
   proof parametricity
     fix A B :: "('a, 'b) nba"
-    assume 1: "(A, B) \<in> \<langle>Id, Id, Id\<rangle> nba_rel"
+    assume 1: "(A, B) \<in> \<langle>Id, Id\<rangle> nba_rel"
     have 2: "(const (Some (2 * card (nodes B), False)) |` initial B,
       const (Some (2 * card (nodes B))) |` initial B, {}) \<in> cs_rel"
       unfolding cs_lr_def cs_st_def in_br_conv by (force simp: restrict_map_def)
@@ -227,13 +225,11 @@ begin
     "('label, 'state) nba \<Rightarrow> 'label \<Rightarrow> 'state items \<Rightarrow> 'state items set" where
     "complement_succ_2 A a \<equiv> ranks_2 A a \<circ> refresh_1"
   definition complement_2 :: "('label, 'state) nba \<Rightarrow> ('label, 'state items) nba" where
-    "complement_2 A \<equiv>
-    \<lparr>
-      alphabet = alphabet A,
-      initial = {const (Some (2 * card (nodes A), False)) |` initial A},
-      succ = complement_succ_2 A,
-      accepting = \<lambda> f. True \<notin> snd ` ran f
-    \<rparr>"
+    "complement_2 A \<equiv> nba
+      (alphabet A)
+      ({const (Some (2 * card (nodes A), False)) |` initial A})
+      (complement_succ_2 A)
+      (\<lambda> f. True \<notin> snd ` ran f)"
 
   lemma ranks_2_refine: "ranks_2 = ranks_1"
   proof (intro ext)
@@ -322,7 +318,7 @@ begin
     qed
   qed
 
-  lemma complement_2_refine: "(complement_2, complement_1) \<in> \<langle>Id, Id, Id\<rangle> nba_rel \<rightarrow> \<langle>Id, Id, Id\<rangle> nba_rel"
+  lemma complement_2_refine: "(complement_2, complement_1) \<in> \<langle>Id, Id\<rangle> nba_rel \<rightarrow> \<langle>Id, Id\<rangle> nba_rel"
     unfolding complement_2_def complement_1_def complement_succ_2_def complement_succ_1_def
     unfolding ranks_2_refine cs_st_def image_def vimage_def ran_def by auto
 
@@ -339,13 +335,11 @@ begin
     "('label, 'state) nba \<Rightarrow> 'label \<Rightarrow> 'state items \<Rightarrow> 'state items set" where
     "complement_succ_3 A a \<equiv> expand_map \<circ> get_3 A \<circ> bounds_3 A a \<circ> refresh_1"
   definition complement_3 :: "('label, 'state) nba \<Rightarrow> ('label, 'state items) nba" where
-    "complement_3 A \<equiv>
-    \<lparr>
-      alphabet = alphabet A,
-      initial = {(Some \<circ> (const (2 * card (nodes A), False))) |` initial A},
-      succ = complement_succ_3 A,
-      accepting = \<lambda> f. \<forall> (p, k, c) \<in> map_to_set f. \<not> c
-    \<rparr>"
+    "complement_3 A \<equiv> nba
+      (alphabet A)
+      ({(Some \<circ> (const (2 * card (nodes A), False))) |` initial A})
+      (complement_succ_3 A)
+      (\<lambda> f. \<forall> (p, k, c) \<in> map_to_set f. \<not> c)"
 
   lemma bounds_3_dom[simp]: "dom (bounds_3 A a f) = UNION (dom f) (succ A a)"
     unfolding bounds_3_def Let_def dom_def by (force split: if_splits)
@@ -387,7 +381,7 @@ begin
   lemma complement_accepting_3_refine: "True \<notin> snd ` ran f \<longleftrightarrow> (\<forall> (p, k, c) \<in> map_to_set f. \<not> c)"
     unfolding map_to_set_def ran_def by auto
 
-  lemma complement_3_refine: "(complement_3, complement_2) \<in> \<langle>Id, Id, Id\<rangle> nba_rel \<rightarrow> \<langle>Id, Id, Id\<rangle> nba_rel"
+  lemma complement_3_refine: "(complement_3, complement_2) \<in> \<langle>Id, Id\<rangle> nba_rel \<rightarrow> \<langle>Id, Id\<rangle> nba_rel"
     unfolding complement_3_def complement_2_def
     unfolding complement_succ_3_refine complement_initial_3_refine complement_accepting_3_refine
     by auto
@@ -650,7 +644,7 @@ begin
     fixes Ai
     fixes ai
     fixes pi
-    assumes Ai: "(Ai, A) \<in> \<langle>Id, Id, Id\<rangle> nbai_nba_rel"
+    assumes Ai: "(Ai, A) \<in> \<langle>Id, Id\<rangle> nbai_nba_rel"
     assumes ai: "(ai, a) \<in> Id"
     assumes pi[autoref_rules]: "(pi, p) \<in> state_rel"
   begin
@@ -676,7 +670,7 @@ begin
 
   lemma complement_succ_6_refine:
     "(RETURN \<circ>\<circ>\<circ> complement_succ_6, complement_succ_5) \<in>
-      \<langle>Id, Id, Id\<rangle> nbai_nba_rel \<rightarrow> Id \<rightarrow> state_rel \<rightarrow>
+      \<langle>Id, Id\<rangle> nbai_nba_rel \<rightarrow> Id \<rightarrow> state_rel \<rightarrow>
       \<langle>\<langle>state_rel\<rangle> list_set_rel\<rangle> nres_rel"
     using complement_succ_6.refine unfolding comp_apply by parametricity
 
@@ -684,7 +678,7 @@ begin
     fixes A :: "('label, nat) nba"
     fixes Ai
     fixes n ni :: nat
-    assumes Ai: "(Ai, A) \<in> \<langle>Id, Id, Id\<rangle> nbai_nba_rel"
+    assumes Ai: "(Ai, A) \<in> \<langle>Id, Id\<rangle> nbai_nba_rel"
     assumes ni[autoref_rules]: "(ni, n) \<in> Id"
   begin
 
@@ -707,27 +701,25 @@ begin
   concrete_definition complement_accepting_6 uses complement_accepting_6
 
   definition complement_6 :: "('label, nat) nbai \<Rightarrow> nat \<Rightarrow> ('label, state) nbai" where
-    "complement_6 Ai ni \<equiv>
-    \<lparr>
-      alphabeti = alphabeti Ai,
-      initiali = complement_initial_6 Ai ni,
-      succi = complement_succ_6 Ai,
-      acceptingi = complement_accepting_6
-    \<rparr>"
+    "complement_6 Ai ni \<equiv> nbai
+      (alphabeti Ai)
+      (complement_initial_6 Ai ni)
+      (complement_succ_6 Ai)
+      (complement_accepting_6)"
 
   lemma complement_6_refine[autoref_rules]:
-    assumes "(Ai, A) \<in> \<langle>Id, Id, Id\<rangle> nbai_nba_rel"
+    assumes "(Ai, A) \<in> \<langle>Id, Id\<rangle> nbai_nba_rel"
     assumes "(ni,
       (OP card ::: \<langle>Id\<rangle> ahs_rel bhc \<rightarrow> nat_rel) $
-      ((OP nodes ::: \<langle>Id, Id, Id\<rangle> nbai_nba_rel \<rightarrow> \<langle>Id\<rangle> ahs_rel bhc) $ A)) \<in> nat_rel"
+      ((OP nodes ::: \<langle>Id, Id\<rangle> nbai_nba_rel \<rightarrow> \<langle>Id\<rangle> ahs_rel bhc) $ A)) \<in> nat_rel"
     shows "(complement_6 Ai ni, (OP complement_3 :::
-      \<langle>Id, Id, Id\<rangle> nbai_nba_rel \<rightarrow> \<langle>Id, state_rel, Id\<rangle> nbai_nba_rel) $ A) \<in> \<langle>Id, state_rel, Id\<rangle> nbai_nba_rel"
+      \<langle>Id, Id\<rangle> nbai_nba_rel \<rightarrow> \<langle>Id, state_rel\<rangle> nbai_nba_rel) $ A) \<in> \<langle>Id, state_rel\<rangle> nbai_nba_rel"
   proof -
     note complement_succ_6_refine
     also note complement_succ_5_refine
     also note complement_succ_4_refine
     finally have 1: "(complement_succ_6, complement_succ_3) \<in>
-      \<langle>Id, Id, Id\<rangle> nbai_nba_rel \<rightarrow> Id \<rightarrow> state_rel \<rightarrow> \<langle>state_rel\<rangle> list_set_rel"
+      \<langle>Id, Id\<rangle> nbai_nba_rel \<rightarrow> Id \<rightarrow> state_rel \<rightarrow> \<langle>state_rel\<rangle> list_set_rel"
       unfolding nres_rel_comp unfolding nres_rel_def unfolding fun_rel_def by auto
     show ?thesis
       unfolding complement_6_def complement_3_def
@@ -737,24 +729,24 @@ begin
   qed
 
   theorem complement_6_correct:
-    assumes "nbai A" "finite (nodes (nba A))"
-    shows "language (nba (complement_6 A (card (nodes (nba A))))) =
-      streams (alphabet (nba A)) - language (nba A)"
+    assumes "nbai_invar A" "finite (nodes (nbai_nba A))"
+    shows "language (nbai_nba (complement_6 A (card (nodes (nbai_nba A))))) =
+      streams (alphabet (nbai_nba A)) - language (nbai_nba A)"
   proof -
     let ?I = "\<langle>\<langle>Id\<rangle> stream_rel\<rangle> set_rel"
-    let ?n = "card (nodes (nba A))"
-    have 1: "(A, nba A) \<in> \<langle>Id, Id, Id\<rangle> nbai_nba_rel"
+    let ?n = "card (nodes (nbai_nba A))"
+    have 1: "(A, nbai_nba A) \<in> \<langle>Id, Id\<rangle> nbai_nba_rel"
       unfolding nbai_nba_br in_br_conv using assms(1) by auto
-    have "(language (nba (complement_6 A ?n)), language (id (complement_3 (nba A)))) \<in> ?I"
+    have "(language (nbai_nba (complement_6 A ?n)), language (id (complement_3 (nbai_nba A)))) \<in> ?I"
       using complement_6_refine 1 by parametricity auto
-    also have "language (id (complement_3 (nba A))) = language (complement_3 (nba A))" by simp
-    also have "(language (complement_3 (nba A)), language (complement_2 (nba A))) \<in> ?I"
+    also have "language (id (complement_3 (nbai_nba A))) = language (complement_3 (nbai_nba A))" by simp
+    also have "(language (complement_3 (nbai_nba A)), language (complement_2 (nbai_nba A))) \<in> ?I"
       using complement_3_refine by parametricity auto
-    also have "(language (complement_2 (nba A)), language (complement_1 (nba A))) \<in> ?I"
+    also have "(language (complement_2 (nbai_nba A)), language (complement_1 (nbai_nba A))) \<in> ?I"
       using complement_2_refine by parametricity auto
-    also have "(language (complement_1 (nba A)), language (complement (nba A))) \<in> ?I"
+    also have "(language (complement_1 (nbai_nba A)), language (complement (nbai_nba A))) \<in> ?I"
       using complement_1_refine by parametricity auto
-    also have "language (complement (nba A)) = streams (alphabet (nba A)) - language (nba A)"
+    also have "language (complement (nbai_nba A)) = streams (alphabet (nbai_nba A)) - language (nbai_nba A)"
       using complement_language assms(2) by this
     finally show ?thesis by simp
   qed
