thys/Transition_Systems_and_Automata/Automata/NBA_Implement.thy
@@ -6,73 +6,80 @@ imports
   "../Basic/Implement"
 begin
 
-  record ('label, 'state) nbai =
-    alphabeti :: "'label list"
-    initiali :: "'state list"
-    succi :: "'label \<Rightarrow> 'state \<Rightarrow> 'state list"
-    acceptingi :: "'state \<Rightarrow> bool"
+  datatype ('label, 'state) nbai = nbai
+    (alphabeti: "'label list")
+    (initiali: "'state list")
+    (succi: "'label \<Rightarrow> 'state \<Rightarrow> 'state list")
+    (acceptingi: "'state \<Rightarrow> bool")
 
-  definition nbai_rel :: "('label\<^sub>1 \<times> 'label\<^sub>2) set \<Rightarrow> ('state\<^sub>1 \<times> 'state\<^sub>2) set \<Rightarrow> ('more\<^sub>1 \<times> 'more\<^sub>2) set \<Rightarrow>
-    (('label\<^sub>1, 'state\<^sub>1, 'more\<^sub>1) nbai_scheme \<times> ('label\<^sub>2, 'state\<^sub>2, 'more\<^sub>2) nbai_scheme) set" where
-    [to_relAPP]: "nbai_rel L S M \<equiv> {(A\<^sub>1, A\<^sub>2).
+  definition nbai_rel :: "('label\<^sub>1 \<times> 'label\<^sub>2) set \<Rightarrow> ('state\<^sub>1 \<times> 'state\<^sub>2) set \<Rightarrow>
+    (('label\<^sub>1, 'state\<^sub>1) nbai \<times> ('label\<^sub>2, 'state\<^sub>2) nbai) set" where
+    [to_relAPP]: "nbai_rel L S \<equiv> {(A\<^sub>1, A\<^sub>2).
       (alphabeti A\<^sub>1, alphabeti A\<^sub>2) \<in> \<langle>L\<rangle> list_rel \<and>
       (initiali A\<^sub>1, initiali A\<^sub>2) \<in> \<langle>S\<rangle> list_rel \<and>
       (succi A\<^sub>1, succi A\<^sub>2) \<in> L \<rightarrow> S \<rightarrow> \<langle>S\<rangle> list_rel \<and>
-      (acceptingi A\<^sub>1, acceptingi A\<^sub>2) \<in> S \<rightarrow> bool_rel \<and>
-      (nbai.more A\<^sub>1, nbai.more A\<^sub>2) \<in> M}"
+      (acceptingi A\<^sub>1, acceptingi A\<^sub>2) \<in> S \<rightarrow> bool_rel}"
 
   lemma nbai_param[param]:
-    "(nbai_ext, nbai_ext) \<in> \<langle>L\<rangle> list_rel \<rightarrow> \<langle>S\<rangle> list_rel \<rightarrow> (L \<rightarrow> S \<rightarrow> \<langle>S\<rangle> list_rel) \<rightarrow>
-      (S \<rightarrow> bool_rel) \<rightarrow> M \<rightarrow> \<langle>L, S, M\<rangle> nbai_rel"
-    "(alphabeti, alphabeti) \<in> \<langle>L, S, M\<rangle> nbai_rel \<rightarrow> \<langle>L\<rangle> list_rel"
-    "(initiali, initiali) \<in> \<langle>L, S, M\<rangle> nbai_rel \<rightarrow> \<langle>S\<rangle> list_rel"
-    "(succi, succi) \<in> \<langle>L, S, M\<rangle> nbai_rel \<rightarrow> L \<rightarrow> S \<rightarrow> \<langle>S\<rangle> list_rel"
-    "(acceptingi, acceptingi) \<in> \<langle>L, S, M\<rangle> nbai_rel \<rightarrow> (S \<rightarrow> bool_rel)"
-    "(nbai.more, nbai.more) \<in> \<langle>L, S, M\<rangle> nbai_rel \<rightarrow> M"
+    "(nbai, nbai) \<in> \<langle>L\<rangle> list_rel \<rightarrow> \<langle>S\<rangle> list_rel \<rightarrow> (L \<rightarrow> S \<rightarrow> \<langle>S\<rangle> list_rel) \<rightarrow>
+      (S \<rightarrow> bool_rel) \<rightarrow> \<langle>L, S\<rangle> nbai_rel"
+    "(alphabeti, alphabeti) \<in> \<langle>L, S\<rangle> nbai_rel \<rightarrow> \<langle>L\<rangle> list_rel"
+    "(initiali, initiali) \<in> \<langle>L, S\<rangle> nbai_rel \<rightarrow> \<langle>S\<rangle> list_rel"
+    "(succi, succi) \<in> \<langle>L, S\<rangle> nbai_rel \<rightarrow> L \<rightarrow> S \<rightarrow> \<langle>S\<rangle> list_rel"
+    "(acceptingi, acceptingi) \<in> \<langle>L, S\<rangle> nbai_rel \<rightarrow> (S \<rightarrow> bool_rel)"
     unfolding nbai_rel_def fun_rel_def by auto
 
-  definition nbai_nba_rel :: "('label\<^sub>1 \<times> 'label\<^sub>2) set \<Rightarrow> ('state\<^sub>1 \<times> 'state\<^sub>2) set \<Rightarrow> ('more\<^sub>1 \<times> 'more\<^sub>2) set \<Rightarrow>
-    (('label\<^sub>1, 'state\<^sub>1, 'more\<^sub>1) nbai_scheme \<times> ('label\<^sub>2, 'state\<^sub>2, 'more\<^sub>2) nba_scheme) set" where
-    [to_relAPP]: "nbai_nba_rel L S M \<equiv> {(A\<^sub>1, A\<^sub>2).
+  definition nbai_nba_rel :: "('label\<^sub>1 \<times> 'label\<^sub>2) set \<Rightarrow> ('state\<^sub>1 \<times> 'state\<^sub>2) set \<Rightarrow>
+    (('label\<^sub>1, 'state\<^sub>1) nbai \<times> ('label\<^sub>2, 'state\<^sub>2) nba) set" where
+    [to_relAPP]: "nbai_nba_rel L S \<equiv> {(A\<^sub>1, A\<^sub>2).
       (alphabeti A\<^sub>1, alphabet A\<^sub>2) \<in> \<langle>L\<rangle> list_set_rel \<and>
       (initiali A\<^sub>1, initial A\<^sub>2) \<in> \<langle>S\<rangle> list_set_rel \<and>
       (succi A\<^sub>1, succ A\<^sub>2) \<in> L \<rightarrow> S \<rightarrow> \<langle>S\<rangle> list_set_rel \<and>
-      (acceptingi A\<^sub>1, accepting A\<^sub>2) \<in> S \<rightarrow> bool_rel \<and>
-      (nbai.more A\<^sub>1, nba.more A\<^sub>2) \<in> M}"
+      (acceptingi A\<^sub>1, accepting A\<^sub>2) \<in> S \<rightarrow> bool_rel}"
 
   lemma nbai_nba_param[param]:
-    "(nbai_ext, nba_ext) \<in> \<langle>L\<rangle> list_set_rel \<rightarrow> \<langle>S\<rangle> list_set_rel \<rightarrow> (L \<rightarrow> S \<rightarrow> \<langle>S\<rangle> list_set_rel) \<rightarrow>
-      (S \<rightarrow> bool_rel) \<rightarrow> M \<rightarrow> \<langle>L, S, M\<rangle> nbai_nba_rel"
-    "(alphabeti, alphabet) \<in> \<langle>L, S, M\<rangle> nbai_nba_rel \<rightarrow> \<langle>L\<rangle> list_set_rel"
-    "(initiali, initial) \<in> \<langle>L, S, M\<rangle> nbai_nba_rel \<rightarrow> \<langle>S\<rangle> list_set_rel"
-    "(succi, succ) \<in> \<langle>L, S, M\<rangle> nbai_nba_rel \<rightarrow> L \<rightarrow> S \<rightarrow> \<langle>S\<rangle> list_set_rel"
-    "(acceptingi, accepting) \<in> \<langle>L, S, M\<rangle> nbai_nba_rel \<rightarrow> S \<rightarrow> bool_rel"
-    "(nbai.more, nba.more) \<in> \<langle>L, S, M\<rangle> nbai_nba_rel \<rightarrow> M"
+    "(nbai, nba) \<in> \<langle>L\<rangle> list_set_rel \<rightarrow> \<langle>S\<rangle> list_set_rel \<rightarrow> (L \<rightarrow> S \<rightarrow> \<langle>S\<rangle> list_set_rel) \<rightarrow>
+      (S \<rightarrow> bool_rel) \<rightarrow> \<langle>L, S\<rangle> nbai_nba_rel"
+    "(alphabeti, alphabet) \<in> \<langle>L, S\<rangle> nbai_nba_rel \<rightarrow> \<langle>L\<rangle> list_set_rel"
+    "(initiali, initial) \<in> \<langle>L, S\<rangle> nbai_nba_rel \<rightarrow> \<langle>S\<rangle> list_set_rel"
+    "(succi, succ) \<in> \<langle>L, S\<rangle> nbai_nba_rel \<rightarrow> L \<rightarrow> S \<rightarrow> \<langle>S\<rangle> list_set_rel"
+    "(acceptingi, accepting) \<in> \<langle>L, S\<rangle> nbai_nba_rel \<rightarrow> S \<rightarrow> bool_rel"
     unfolding nbai_nba_rel_def fun_rel_def by auto
 
-  definition nba :: "('label, 'state, 'more) nbai_scheme \<Rightarrow> ('label, 'state, 'more) nba_scheme" where
-    "nba A \<equiv> \<lparr> alphabet = set (alphabeti A), initial = set (initiali A),
-      succ = \<lambda> a p. set (succi A a p), accepting = acceptingi A, \<dots> = nbai.more A \<rparr>"
-  definition nbai :: "('label, 'state, 'more) nbai_scheme \<Rightarrow> bool" where
-    "nbai A \<equiv> distinct (alphabeti A) \<and> distinct (initiali A) \<and> (\<forall> a p. distinct (succi A a p))"
+  definition nbai_nba :: "('label, 'state) nbai \<Rightarrow> ('label, 'state) nba" where
+    "nbai_nba A \<equiv> nba (set (alphabeti A)) (set (initiali A)) (\<lambda> a p. set (succi A a p)) (acceptingi A)"
+  definition nbai_invar :: "('label, 'state) nbai \<Rightarrow> bool" where
+    "nbai_invar A \<equiv> distinct (alphabeti A) \<and> distinct (initiali A) \<and> (\<forall> a p. distinct (succi A a p))"
 
-  lemma nbai_nba_br: "\<langle>Id, Id, Id\<rangle> nbai_nba_rel = br nba nbai"
-    unfolding nbai_nba_rel_def nba_def nbai_def
-    by (fastforce intro!: nba.equality simp: fun_rel_def in_br_conv list_set_rel_def)
-
-  lemma ba_id_param[param]: "(nba, id) \<in> \<langle>L, S, M\<rangle> nbai_nba_rel \<rightarrow> \<langle>L, S, M\<rangle> nba_rel"
+  lemma nbai_nba_id_param[param]: "(nbai_nba, id) \<in> \<langle>L, S\<rangle> nbai_nba_rel \<rightarrow> \<langle>L, S\<rangle> nba_rel"
   proof
     fix Ai A
-    assume 1: "(Ai, A) \<in> \<langle>L, S, M\<rangle> nbai_nba_rel"
-    have 2: "nba Ai = \<lparr> alphabet = set (alphabeti Ai), initial = set (initiali Ai),
-      succ = \<lambda> a p. set (succi Ai a p), accepting = acceptingi Ai, \<dots> = nbai.more Ai \<rparr>"
-      unfolding nba_def by rule
-    have 3: "id A = \<lparr> alphabet = id (alphabet A), initial = id (initial A),
-      succ = \<lambda> a p. id (succ A a p), accepting = accepting A, \<dots> = nba.more A \<rparr>" by simp
-    show "(nba Ai, id A) \<in> \<langle>L, S, M\<rangle> nba_rel" unfolding 2 3 using 1 by parametricity
+    assume 1: "(Ai, A) \<in> \<langle>L, S\<rangle> nbai_nba_rel"
+    have 2: "nbai_nba Ai = nba (set (alphabeti Ai)) (set (initiali Ai))
+      (\<lambda> a p. set (succi Ai a p)) (acceptingi Ai)" unfolding nbai_nba_def by rule
+    have 3: "id A = nba (id (alphabet A)) (id (initial A))
+      (\<lambda> a p. id (succ A a p)) (accepting A)" by simp
+    show "(nbai_nba Ai, id A) \<in> \<langle>L, S\<rangle> nba_rel" unfolding 2 3 using 1 by parametricity
+  qed
+
+  lemma nbai_nba_br: "\<langle>Id, Id\<rangle> nbai_nba_rel = br nbai_nba nbai_invar"
+  proof safe
+    show "(A, B) \<in> \<langle>Id, Id\<rangle> nbai_nba_rel" if "(A, B) \<in> br nbai_nba nbai_invar"
+      for A and B :: "('a, 'b) nba"
+      using that unfolding nbai_nba_rel_def nbai_nba_def nbai_invar_def
+      by (auto simp: in_br_conv list_set_rel_def)
+    show "(A, B) \<in> br nbai_nba nbai_invar" if "(A, B) \<in> \<langle>Id, Id\<rangle> nbai_nba_rel"
+      for A and B :: "('a, 'b) nba"
+    proof -
+      have 1: "(nbai_nba A, id B) \<in> \<langle>Id, Id\<rangle> nba_rel" using that by parametricity
+      have 2: "nbai_invar A"
+        using nbai_nba_param(2 - 5)[param_fo, OF that]
+        by (auto simp: in_br_conv list_set_rel_def nbai_invar_def)
+      show ?thesis using 1 2 unfolding in_br_conv by auto
+    qed
   qed
 
   (* TODO: take a look at Digraph_Impl setup to make synthesizing whole nbai/bae possible *)
-  lemmas [autoref_rules] = nbai_nba_param(2-6)
+  lemmas [autoref_rules] = nbai_nba_param(2-5)
 
 end
