thys/Transition_Systems_and_Automata/Automata/NBA_Translate.thy
@@ -13,19 +13,17 @@ begin
 
   section {* Image on Explicit Automata *}
 
-  definition nbae_image where "nbae_image f A \<equiv> \<lparr> alphabete = alphabete A, initiale = f ` initiale A,
-    transe = (\<lambda> (p, a, q). (f p, a, f q)) ` transe A, acceptinge = f ` acceptinge A, \<dots> = nbae.more A \<rparr>"
+  definition nbae_image where "nbae_image f A \<equiv> nbae (alphabete A) (f ` initiale A)
+    ((\<lambda> (p, a, q). (f p, a, f q)) ` transe A) (f ` acceptinge A)"
 
-  lemma nbae_image_param[param]: "(nbae_image, nbae_image) \<in> (S \<rightarrow> T) \<rightarrow> \<langle>L, S, M\<rangle> nbae_rel \<rightarrow> \<langle>L, T, M\<rangle> nbae_rel"
+  lemma nbae_image_param[param]: "(nbae_image, nbae_image) \<in> (S \<rightarrow> T) \<rightarrow> \<langle>L, S\<rangle> nbae_rel \<rightarrow> \<langle>L, T\<rangle> nbae_rel"
     unfolding nbae_image_def by parametricity
 
   lemma nbae_image_id[simp]: "nbae_image id = id" unfolding nbae_image_def by auto
-  lemma nbae_image_nba_nbae: "nbae_image f (nba_nbae A) = \<lparr>
-    alphabete = alphabet A,
-    initiale = f ` initial A,
-    transe = (\<Union> p \<in> nodes A. \<Union> a \<in> alphabet A. f ` {p} \<times> {a} \<times> f ` succ A a p),
-    acceptinge = f ` {p \<in> nodes A. accepting A p},
-    \<dots> = nba.more A \<rparr>"
+  lemma nbae_image_nba_nbae: "nbae_image f (nba_nbae A) = nbae
+    (alphabet A) (f ` initial A)
+    (\<Union> p \<in> nodes A. \<Union> a \<in> alphabet A. f ` {p} \<times> {a} \<times> f ` succ A a p)
+    (f ` {p \<in> nodes A. accepting A p})"
     unfolding nba_nbae_def nbae_image_def nbae.simps Set.filter_def by force
 
   section {* Exploration and Translation *}
@@ -96,7 +94,7 @@ begin
       by auto
   qed
 
-  definition to_nbaei :: "('state, 'label, 'more) nba_scheme \<Rightarrow> ('state, 'label, 'more) nba_scheme"
+  definition to_nbaei :: "('state, 'label) nba \<Rightarrow> ('state, 'label) nba"
     where "to_nbaei \<equiv> id"
 
   (* TODO: make separate implementations for "nba_nbae" and "op_set_enumerate \<bind> nbae_image" *)
@@ -106,7 +104,7 @@ begin
     assumes [autoref_ga_rules]: "is_bounded_hashcode S seq bhc"
     assumes [autoref_ga_rules]: "is_valid_def_hm_size TYPE('statei) hms"
     assumes [autoref_rules]: "(seq, HOL.eq) \<in> S \<rightarrow> S \<rightarrow> bool_rel"
-    assumes [autoref_rules]: "(Ai, A) \<in> \<langle>L, S, M\<rangle> nbai_nba_rel"
+    assumes [autoref_rules]: "(Ai, A) \<in> \<langle>L, S\<rangle> nbai_nba_rel"
     shows "(?f :: ?'a, do {
         let N = nodes A;
         f \<leftarrow> op_set_enumerate N;
@@ -114,8 +112,8 @@ begin
         ASSERT (\<forall> p \<in> initial A. f p \<noteq> None);
         ASSERT (\<forall> p \<in> dom f. \<forall> a \<in> alphabet A. \<forall> q \<in> succ A a p. f q \<noteq> None);
         T \<leftarrow> trans_algo N (alphabet A) (succ A) (\<lambda> x. the (f x));
-        RETURN \<lparr> alphabete = alphabet A, initiale = (\<lambda> x. the (f x)) ` initial A,
-          transe = T, acceptinge = (\<lambda> x. the (f x)) ` {p \<in> N. accepting A p}, \<dots> = nba.more A \<rparr>
+        RETURN (nbae (alphabet A) ((\<lambda> x. the (f x)) ` initial A) T
+          ((\<lambda> x. the (f x)) ` {p \<in> N. accepting A p}))
       }) \<in> ?R"
     unfolding trans_algo_def by (autoref_monadic (plain))
   concrete_definition to_nbaei_impl uses to_nbaei_impl[unfolded autoref_tag_defs CAST_def id_apply]
@@ -125,11 +123,11 @@ begin
     assumes "is_bounded_hashcode S seq bhc"
     assumes "is_valid_def_hm_size TYPE('statei) hms"
     assumes "(seq, HOL.eq) \<in> S \<rightarrow> S \<rightarrow> bool_rel"
-    assumes "(Ai, A) \<in> \<langle>L, S, M\<rangle> nbai_nba_rel"
+    assumes "(Ai, A) \<in> \<langle>L, S\<rangle> nbai_nba_rel"
     shows "(RETURN (to_nbaei_impl seq bhc hms Ai), do {
         f \<leftarrow> op_set_enumerate (nodes A);
         RETURN (nbae_image (the \<circ> f) (nba_nbae A))
-      }) \<in> \<langle>\<langle>L, nat_rel, M\<rangle> nbaei_nbae_rel\<rangle> nres_rel"
+      }) \<in> \<langle>\<langle>L, nat_rel\<rangle> nbaei_nbae_rel\<rangle> nres_rel"
   proof -
     have 1: "finite (alphabet A)"
       using nbai_nba_param(2)[param_fo, OF assms(5)] list_set_rel_finite
@@ -142,21 +140,18 @@ begin
         ASSERT (\<forall> p \<in> initial A. f p \<noteq> None);
         ASSERT (\<forall> p \<in> dom f. \<forall> a \<in> alphabet A. \<forall> q \<in> succ A a p. f q \<noteq> None);
         T \<leftarrow> trans_algo N (alphabet A) (succ A) (\<lambda> x. the (f x));
-        RETURN \<lparr> alphabete = alphabet A, initiale = (\<lambda> x. the (f x)) ` initial A,
-          transe = T, acceptinge = (\<lambda>x. the (f x)) ` {p \<in> N. accepting A p}, \<dots> = nba.more A \<rparr>
+        RETURN (nbae (alphabet A) ((\<lambda> x. the (f x)) ` initial A) T ((\<lambda> x. the (f x)) ` {p \<in> N. accepting A p}))
       }, do {
         f \<leftarrow> op_set_enumerate (nodes A);
         T \<leftarrow> SPEC (HOL.eq (trans_spec A (\<lambda> x. the (f x))));
-        RETURN \<lparr> alphabete = alphabet A, initiale = (\<lambda> x. the (f x)) ` initial A,
-          transe = T, acceptinge = (\<lambda>x. the (f x)) ` {p \<in> nodes A. accepting A p}, \<dots> = nba.more A \<rparr>
+        RETURN (nbae (alphabet A) ((\<lambda> x. the (f x)) ` initial A) T ((\<lambda> x. the (f x)) ` {p \<in> nodes A. accepting A p}))
       }) \<in> \<langle>Id\<rangle> nres_rel"
       unfolding Let_def comp_apply op_set_enumerate_def using assms(1) 1
       by (refine_vcg vcg0[OF trans_algo_refine]) (auto intro!: inj_on_map_the[unfolded comp_apply])
     also have "(do {
         f \<leftarrow> op_set_enumerate (nodes A);
         T \<leftarrow> SPEC (HOL.eq (trans_spec A (\<lambda> x. the (f x))));
-        RETURN \<lparr> alphabete = alphabet A, initiale = (\<lambda> x. the (f x)) ` initial A,
-          transe = T, acceptinge = (\<lambda>x. the (f x)) ` {p \<in> nodes A. accepting A p}, \<dots> = nba.more A \<rparr>
+        RETURN (nbae (alphabet A) ((\<lambda> x. the (f x)) ` initial A) T ((\<lambda> x. the (f x)) ` {p \<in> nodes A. accepting A p}))
       },  do {
         f \<leftarrow> op_set_enumerate (nodes A);
         RETURN (nbae_image (the \<circ> f) (nba_nbae A))
@@ -170,20 +165,19 @@ begin
     fixes Ai A
     fixes seq bhc hms
     fixes S :: "('statei \<times> 'state) set"
-    fixes M
     assumes a: "finite (nodes A)"
     assumes b: "is_bounded_hashcode S seq bhc"
     assumes c: "is_valid_def_hm_size TYPE('statei) hms"
     assumes d: "(seq, HOL.eq) \<in> S \<rightarrow> S \<rightarrow> bool_rel"
-    assumes e: "(Ai, A) \<in> \<langle>Id, S, M\<rangle> nbai_nba_rel"
+    assumes e: "(Ai, A) \<in> \<langle>Id, S\<rangle> nbai_nba_rel"
   begin
 
     definition f' where "f' \<equiv> SOME f'.
-      (to_nbaei_impl seq bhc hms Ai, nbae_image (the \<circ> f') (nba_nbae A)) \<in> \<langle>Id, nat_rel, M\<rangle> nbaei_nbae_rel \<and>
+      (to_nbaei_impl seq bhc hms Ai, nbae_image (the \<circ> f') (nba_nbae A)) \<in> \<langle>Id, nat_rel\<rangle> nbaei_nbae_rel \<and>
       dom f' = nodes A \<and> inj_on f' (nodes A)"
 
     lemma 1: "\<exists> f'. (to_nbaei_impl seq bhc hms Ai, nbae_image (the \<circ> f') (nba_nbae A)) \<in>
-      \<langle>Id, nat_rel, M\<rangle> nbaei_nbae_rel \<and> dom f' = nodes A \<and> inj_on f' (nodes A)"
+      \<langle>Id, nat_rel\<rangle> nbaei_nbae_rel \<and> dom f' = nodes A \<and> inj_on f' (nodes A)"
       using to_nbaei_impl_refine''[
         OF a b c d e,
         unfolded op_set_enumerate_def bind_RES_RETURN_eq,
@@ -192,7 +186,7 @@ begin
       by force
 
     lemma f'_refine: "(to_nbaei_impl seq bhc hms Ai, nbae_image (the \<circ> f') (nba_nbae A)) \<in>
-      \<langle>Id, nat_rel, M\<rangle> nbaei_nbae_rel" using someI_ex[OF 1, folded f'_def] by auto
+      \<langle>Id, nat_rel\<rangle> nbaei_nbae_rel" using someI_ex[OF 1, folded f'_def] by auto
     lemma f'_dom: "dom f' = nodes A" using someI_ex[OF 1, folded f'_def] by auto
     lemma f'_inj: "inj_on f' (nodes A)" using someI_ex[OF 1, folded f'_def] by auto
 
@@ -222,14 +216,14 @@ begin
     lemma [param]: "(g, id) \<in> rel \<rightarrow> Id_on (Range rel)" unfolding rel_inv_def by (auto simp: in_br_conv)
 
     lemma to_nbaei_impl_refine':
-      "(to_nbaei_impl seq bhc hms Ai, to_nbaei A) \<in> \<langle>Id_on (alphabet A), rel, M\<rangle> nbaei_nba_rel"
+      "(to_nbaei_impl seq bhc hms Ai, to_nbaei A) \<in> \<langle>Id_on (alphabet A), rel\<rangle> nbaei_nba_rel"
     proof -
-      have "(nbae_nba (nbae (to_nbaei_impl seq bhc hms Ai)), nbae_nba (id (nbae_image f (nba_nbae A)))) \<in>
-        \<langle>Id, nat_rel, M\<rangle> nba_rel" using f'_refine[folded f_def] by parametricity auto
+      have "(nbae_nba (nbaei_nbae (to_nbaei_impl seq bhc hms Ai)), nbae_nba (id (nbae_image f (nba_nbae A)))) \<in>
+        \<langle>Id, nat_rel\<rangle> nba_rel" using f'_refine[folded f_def] by parametricity auto
       also have "(nbae_nba (id (nbae_image f (nba_nbae A))), nbae_nba (id (nbae_image id (nba_nbae A)))) \<in>
-        \<langle>Id_on (alphabet A), rel, Id\<rangle> nba_rel" using nba_rel_eq by parametricity auto
+        \<langle>Id_on (alphabet A), rel\<rangle> nba_rel" using nba_rel_eq by parametricity auto
       also have "nbae_nba (id (nbae_image id (nba_nbae A))) = (nbae_nba \<circ> nba_nbae) A" by simp
-      also have "(\<dots>, id A) \<in> \<langle>Id_on (alphabet A), Id_on (nodes A), Id\<rangle> nba_rel" by parametricity
+      also have "(\<dots>, id A) \<in> \<langle>Id_on (alphabet A), Id_on (nodes A)\<rangle> nba_rel" by parametricity
       also have "id A = to_nbaei A" unfolding to_nbaei_def by simp
       finally show ?thesis unfolding nbaei_nba_rel_def by simp
     qed
@@ -247,11 +241,11 @@ begin
       assumes "SIDE_GEN_ALGO (is_bounded_hashcode S seq bhc)"
       assumes "SIDE_GEN_ALGO (is_valid_def_hm_size TYPE('statei) hms)"
       assumes "GEN_OP seq HOL.eq (S \<rightarrow> S \<rightarrow> bool_rel)"
-      assumes "(Ai, A) \<in> \<langle>Id, S, M\<rangle> nbai_nba_rel"
+      assumes "(Ai, A) \<in> \<langle>Id, S\<rangle> nbai_nba_rel"
       shows "(to_nbaei_impl seq bhc hms Ai,
-        (OP to_nbaei ::: \<langle>Id, S, M\<rangle> nbai_nba_rel \<rightarrow>
-        \<langle>Id_on (alphabet A), rel Ai A seq bhc hms M, M\<rangle> nbaei_nba_rel) $ A) \<in>
-        \<langle>Id_on (alphabet A), rel Ai A seq bhc hms M, M\<rangle> nbaei_nba_rel"
+        (OP to_nbaei ::: \<langle>Id, S\<rangle> nbai_nba_rel \<rightarrow>
+        \<langle>Id_on (alphabet A), rel Ai A seq bhc hms\<rangle> nbaei_nba_rel) $ A) \<in>
+        \<langle>Id_on (alphabet A), rel Ai A seq bhc hms\<rangle> nbaei_nba_rel"
       using to_nbaei_impl_refine' assms unfolding autoref_tag_defs by this
 
   end
